code/streaming/Hacl.Streaming.HMAC.Definitions.fst
@@ -22,6 +22,66 @@ let _sync_decl = ()
 
 friend Spec.Agile.HMAC
 friend Spec.HMAC.Incremental
+friend Hacl.HMAC
+
+noextract inline_for_extraction
+val alloca_block: (i: G.erased impl) ->
+  ST.StackInline (b:B.buffer uint8)
+    (requires (fun h ->
+      HS.is_stack_region (HS.get_tip h)))
+    (ensures (fun h0 s h1 ->
+      M.(modifies M.loc_none h0 h1) /\
+      B.frameOf s == HS.get_tip h0 /\
+      B.length s == Spec.Agile.Hash.block_length (alg_of_impl i) /\
+      B.as_seq h1 s == Seq.create (Spec.Agile.Hash.block_length (alg_of_impl i)) (Lib.IntTypes.u8 0) /\
+      B.live h1 s /\
+      B.fresh_loc (M.loc_buffer s) h0 h1))
+
+// This extracts in C without a VLA.
+let alloca_block i =
+  let b = B.alloca (Lib.IntTypes.u8 0) 168ul in
+  assert (D.block_len (alg_of_impl i) `FStar.UInt32.lte` 168ul);
+  let r = B.sub b 0ul (D.block_len (alg_of_impl i)) in
+  let h = ST.get () in
+  assert (B.as_seq h r `S.equal` S.create (Spec.Agile.Hash.block_length (alg_of_impl i)) (Lib.IntTypes.u8 0));
+  r
+
+// TODO: copy-paste from Hacl.HMAC
+inline_for_extraction noextract
+let wrap_key (impl: impl): Hacl.HMAC.wrap_key_st (alg_of_impl impl) =
+fun output key len ->
+  [@inline_let]
+  let a = alg_of_impl impl in
+  [@inline_let] //18-08-02 does *not* prevents unused-but-set-variable warning in C
+  let i = Hacl.HMAC.helper_smtpat a len in
+  let nkey = B.sub output 0ul i in
+  let zeroes = B.sub output i (D.block_len a `FStar.UInt32.sub` i) in
+  (**) assert B.(loc_disjoint (loc_buffer nkey) (loc_buffer zeroes));
+  (**) let h0 = ST.get () in
+  (**) assert (Seq.equal (B.as_seq h0 zeroes) (Seq.create (UInt32.v (D.block_len a `FStar.UInt32.sub` i)) (Lib.IntTypes.u8 0)));
+  if len `FStar.UInt32.lte` D.block_len a then begin
+    B.blit key 0ul nkey 0ul len;
+    let h1 = ST.get () in
+    (**) assert (Seq.equal (B.as_seq h1 zeroes) (B.as_seq h0 zeroes));
+    (**) assert (Seq.equal (B.as_seq h1 nkey) (B.as_seq h0 key));
+    (**) assert (Seq.equal (B.as_seq h1 output) (S.append (B.as_seq h1 nkey) (B.as_seq h1 zeroes)));
+    (**) Seq.lemma_eq_elim (B.as_seq h1 output) (S.append (B.as_seq h1 nkey) (B.as_seq h1 zeroes));
+    (**) assert (B.as_seq h1 output == Spec.Agile.HMAC.wrap a (B.as_seq h0 key))
+  end else begin
+    Hacl.Agile.Hash.hash impl nkey key len;
+    (**) let h1 = ST.get () in
+    (**) assert (Seq.equal (B.as_seq h1 zeroes) (B.as_seq h0 zeroes));
+    (**) assert (Seq.equal (B.as_seq h1 nkey) (Spec.Agile.Hash.hash a (B.as_seq h0 key)));
+    (**) assert (Seq.equal (B.as_seq h1 output) (S.append (B.as_seq h1 nkey) (B.as_seq h1 zeroes)));
+    (**) Seq.lemma_eq_elim (B.as_seq h1 output) (S.append (B.as_seq h1 nkey) (B.as_seq h1 zeroes));
+    (**) assert (B.as_seq h1 output == Spec.Agile.HMAC.wrap a (B.as_seq h0 key))
+  end
 
 let init (i: G.erased index) k buf s =
-  admit ()
+  push_frame ();
+  admit ();
+  let i = Hacl.Agile.Hash.impl_of_state (dfst i) s in
+  let block = alloca_block i in
+  let k, k_len = k in
+  wrap_key i block k !*k_len;
+  pop_frame ()
